Rework RawPointer and add manual instance for `LinearOrder RawPointer`

Bdd/Apply.lean
@@ -20,7 +20,7 @@ def Invariant {n m n' m'} (op : Bool → Bool → Bool) (O_heap : Vector (Node n
   ∃ hh : (∀ i : Fin r.size, RawNode.Bounded i r.heap[i]),
     ∀ (k : (Pointer m × Pointer m')) (p : RawPointer),
       r.cache[k]? = some p →
-      (∀ j h, p = .inr j → (r.heap[j]'h).va.1 =
+      (∀ j h, p = .node j → (r.heap[j]'h).va.1 =
         (k.1.toVarD O_heap (n ⊔ n')) ⊓ (k.2.toVarD U_heap (n ⊔ n'))) ∧
       ∃ hk1 : Bdd.Ordered ⟨O_heap, k.1⟩,
         ∃ hk2 : Bdd.Ordered ⟨U_heap, k.2⟩,
@@ -44,15 +44,15 @@ def cache_get {m m' n n'} (O_root : Pointer m) (U_root : Pointer m') (s : (State
 
 def heap_push {n n' m m'} (O : OBdd n m) (U : OBdd n' m') (N : RawNode (n ⊔ n'))
     (s : State n n' m m') : State n n' m m' × RawPointer :=
-  ⟨⟨s.size + 1, s.heap.push N, s.cache.insert ⟨O.1.root, U.1.root⟩ (.inr s.size)⟩, .inr s.size⟩
+  ⟨⟨s.size + 1, s.heap.push N, s.cache.insert ⟨O.1.root, U.1.root⟩ (.node s.size)⟩, .node s.size⟩
 
 lemma heap_push_aux {n n' m m' op} {O : OBdd n m} {U : OBdd n' m'} {N} (s : (State n n' m m'))
     (inv : Invariant op O.bdd.heap U.bdd.heap s)
     (hNl : ∃ k : Pointer m × Pointer m', s.cache[k]? = some N.lo)
     (hNh : ∃ k : Pointer m × Pointer m', s.cache[k]? = some N.hi)
     (hNv : N.va.1 = O.bdd.root.toVarD O.1.heap (n ⊔ n') ⊓ U.bdd.root.toVarD U.1.heap (n ⊔ n'))
-    (hxl : ∀ j h (_ : N.lo = .inr j), N.va.1 < (s.heap[j]'h).va.1)
-    (hxh : ∀ j h (_ : N.hi = .inr j), N.va.1 < (s.heap[j]'h).va.1)
+    (hxl : ∀ j h (_ : N.lo = .node j), N.va.1 < (s.heap[j]'h).va.1)
+    (hxh : ∀ j h (_ : N.hi = .node j), N.va.1 < (s.heap[j]'h).va.1)
     (hh : ∀ h0 (h1 : Bdd.Ordered _) (I : Vector Bool (max n n')),
       OBdd.evaluate ⟨{ heap := cook_heap (s.heap.push N) h0, root := Pointer.node ⟨s.size, by simp⟩ }, h1⟩ I =
       op (O.evaluate (Vector.cast (by omega) (I.extract 0 n))) (U.evaluate (Vector.cast (by omega) (I.extract 0 n')))) :
@@ -73,8 +73,8 @@ lemma heap_push_aux {n n' m m' op} {O : OBdd n m} {U : OBdd n' m'} {N} (s : (Sta
       rw [this]
       exact hN
   use this
-  have hb : RawPointer.Bounded (s.size + 1) (Sum.inr s.size) := by
-    simp only [RawPointer.bounded_inr_iff, Nat.lt_add_one]
+  have hb : RawPointer.Bounded (s.size + 1) (.node s.size) := by
+    simp only [RawPointer.bounded_node_iff, Nat.lt_add_one]
   simp only [heap_push]
   intro k p hp
   rw [Std.HashMap.getElem?_insert] at hp
@@ -89,27 +89,27 @@ lemma heap_push_aux {n n' m m' op} {O : OBdd n m} {U : OBdd n' m'} {N} (s : (Sta
       injection hp with hpe
       subst hpe
       use hb
-      have hoo : Bdd.Ordered ⟨cook_heap (s.heap.push N) this, RawPointer.cook (Sum.inr s.size) hb⟩ := by
-        apply Bdd.ordered_of_low_high_ordered (by rw [RawPointer.cook_inr, Pointer.node.injEq])
+      have hoo : Bdd.Ordered ⟨cook_heap (s.heap.push N) this, RawPointer.cook (.node s.size) hb⟩ := by
+        apply Bdd.ordered_of_low_high_ordered (by rw [RawPointer.cook_node, Pointer.node.injEq])
         · simp only [Bdd.low_eq, cook_heap_eq]
           simp only [Fin.getElem_fin, Vector.getElem_ofFn, Vector.getElem_push_eq]
           rw [cook_low]
           convert push_ordered ho_lo
           rw [cook_heap_eq (hh := this)]; rfl
-        · simp [Nat.succ_eq_add_one, Bdd.var_eq, cook_heap_eq, Bdd.low_eq, RawPointer.cook_inr]
+        · simp [Nat.succ_eq_add_one, Bdd.var_eq, cook_heap_eq, Bdd.low_eq, RawPointer.cook_node]
           cases heq : N.lo with
-          | inl val =>
+          | terminal val =>
             rw [cook_low]
             simp_rw [heq]
-            simp only [RawNode.cook_eq, RawPointer.cook_inl, Pointer.toVar_terminal,
+            simp only [RawNode.cook_eq, RawPointer.cook_terminal, Pointer.toVar_terminal,
               Nat.succ_eq_add_one, Fin.lt_def, Pointer.toVar_node, Fin.getElem_fin,
               Vector.getElem_ofFn, Vector.getElem_push_eq, lt_sup_iff]
             omega
-          | inr val =>
-            rw [heq, RawPointer.bounded_inr_iff] at hb_lo
+          | node val =>
+            rw [heq, RawPointer.bounded_node_iff] at hb_lo
             rw [cook_low]
             simp_rw [heq]
-            simp only [RawNode.cook_eq, RawPointer.cook_inr, Fin.lt_def, Nat.succ_eq_add_one,
+            simp only [RawNode.cook_eq, RawPointer.cook_node, Fin.lt_def, Nat.succ_eq_add_one,
               Pointer.toVar_node, Fin.getElem_fin, Vector.getElem_ofFn, Vector.getElem_push_eq]
             rw [Vector.getElem_push_lt]
             exact hxl _ hb_lo heq
@@ -118,26 +118,26 @@ lemma heap_push_aux {n n' m m' op} {O : OBdd n m} {U : OBdd n' m'} {N} (s : (Sta
           rw [cook_high]
           convert push_ordered ho_hi
           rw [cook_heap_eq (hh := this)]; rfl
-        · simp [Nat.succ_eq_add_one, Bdd.var_eq, cook_heap_eq, Bdd.high_eq, RawPointer.cook_inr]
+        · simp [Nat.succ_eq_add_one, Bdd.var_eq, cook_heap_eq, Bdd.high_eq, RawPointer.cook_node]
           cases heq : N.hi with
-          | inl val =>
+          | terminal val =>
             rw [cook_high]
             simp_rw [heq]
-            simp only [RawPointer.cook_inl, Fin.lt_def, Nat.succ_eq_add_one, Pointer.toVar_node]
+            simp only [RawPointer.cook_terminal, Fin.lt_def, Nat.succ_eq_add_one, Pointer.toVar_node]
             simp only [RawNode.cook_eq, Fin.getElem_fin, Vector.getElem_ofFn, Vector.getElem_push_eq,
               Pointer.toVar_terminal, Nat.succ_eq_add_one, lt_sup_iff]
             omega
-          | inr val =>
-            rw [heq, RawPointer.bounded_inr_iff] at hb_hi
+          | node val =>
+            rw [heq, RawPointer.bounded_node_iff] at hb_hi
             rw [cook_high]
             simp_rw [heq]
-            simp only [RawNode.cook_eq, RawPointer.cook_inr]
+            simp only [RawNode.cook_eq, RawPointer.cook_node]
             simp_rw [Fin.lt_def, Nat.succ_eq_add_one, Pointer.toVar_node, Fin.getElem_fin,
               Vector.getElem_ofFn, Vector.getElem_push_eq]
             rw [Vector.getElem_push_lt]
             exact hxh _ hb_hi heq
       use hoo
-      simp only [OBdd.mk_eq_self, RawPointer.cook_inr] at ⊢ hoo
+      simp only [OBdd.mk_eq_self, RawPointer.cook_node] at ⊢ hoo
       intro I
       apply hh _ hoo
   next heq =>
@@ -169,8 +169,8 @@ lemma heap_push_correct {n n' m m' op} {O : OBdd n m} {U : OBdd n' m'} (N : RawN
     (hNl : ∃ k : Pointer m × Pointer m', s.cache[k]? = some N.lo)
     (hNh : ∃ k : Pointer m × Pointer m', s.cache[k]? = some N.hi)
     (hNv : N.va.1 = O.bdd.root.toVarD O.1.heap (n ⊔ n') ⊓ U.bdd.root.toVarD U.1.heap (n ⊔ n'))
-    (hxl : ∀ j h (_ : N.lo = .inr j), N.va.1 < (s.heap[j]'h).va.1)
-    (hxh : ∀ j h (_ : N.hi = .inr j), N.va.1 < (s.heap[j]'h).va.1)
+    (hxl : ∀ j h (_ : N.lo = .node j), N.va.1 < (s.heap[j]'h).va.1)
+    (hxh : ∀ j h (_ : N.hi = .node j), N.va.1 < (s.heap[j]'h).va.1)
     (hh : ∀ h0 (h1 : Bdd.Ordered _) (I : Vector Bool (max n n')),
             OBdd.evaluate ⟨{ heap := cook_heap (s.heap.push N) h0, root := Pointer.node ⟨s.size, by simp⟩ }, h1⟩ I =
             op (O.evaluate (Vector.cast (by omega) (I.extract 0 n))) (U.evaluate (Vector.cast (by omega) (I.extract 0 n'))))
@@ -209,7 +209,7 @@ lemma heap_push_correct {n n' m m' op} {O : OBdd n m} {U : OBdd n' m'} (N : RawN
 lemma insert_terminal_invariant {n n' m m' op} {O : OBdd n m} {U : OBdd n' m'} {b b'}
     (s0 : State n n' m m') (inv : Invariant op O.bdd.heap U.bdd.heap s0)
     (ho : O.1.root = .terminal b) (hu : U.1.root = .terminal b') :
-    Invariant op O.bdd.heap U.bdd.heap { size := s0.size, heap := s0.heap, cache := s0.cache.insert (O.1.root, U.1.root) (Sum.inl (op b b')) } := by
+    Invariant op O.bdd.heap U.bdd.heap { size := s0.size, heap := s0.heap, cache := s0.cache.insert (O.1.root, U.1.root) (.terminal (op b b')) } := by
   constructor
   intro k p hp
   simp only at hp
@@ -227,8 +227,8 @@ lemma insert_terminal_invariant {n n' m m' op} {O : OBdd n m} {U : OBdd n' m'} {
     use O.2, U.2
     injection hp with hpe
     subst hpe
-    use RawPointer.bounded_inl
-    simp [RawPointer.cook_inl, ho, hu, Bdd.ordered_of_terminal]
+    use RawPointer.bounded_terminal
+    simp [RawPointer.cook_terminal, ho, hu, Bdd.ordered_of_terminal]
   next =>
     constructor
     · exact (inv.2 _ _ hp).1
@@ -410,7 +410,7 @@ def apply_helper {n m n' m'} (op : (Bool → Bool → Bool)) (O : OBdd n m) (U :
     | .terminal b =>
       match U_root_def : U.1.root with
       | .terminal b' =>
-        ⟨⟨s0.size, s0.heap, s0.cache.insert ⟨O.1.root, U.1.root⟩ (.inl (op b b'))⟩, .inl (op b b')⟩
+        ⟨⟨s0.size, s0.heap, s0.cache.insert ⟨O.1.root, U.1.root⟩ (.terminal (op b b'))⟩, .terminal (op b b')⟩
       | .node j' =>
         let ⟨sl, rl⟩ := apply_helper op O (U.low U_root_def) s0
         let ⟨sh, rh⟩ := apply_helper op O (U.high U_root_def) sl
@@ -504,7 +504,7 @@ lemma apply_helper_correct {n m n' m'} (op : (Bool → Bool → Bool)) (O : OBdd
         intro j hj1 hj2
         have := (hhp _).1 _ hl
         rw [hj2] at this
-        have that := (invh.2 _ (.inr j) this).1 _ hj1 rfl
+        have that := (invh.2 _ (.node j) this).1 _ hj1 rfl
         simp only at that
         rw [that]
         exact aux_lt1_low O_root_def U_root_def
@@ -611,7 +611,7 @@ lemma apply_helper_correct {n m n' m'} (op : (Bool → Bool → Bool)) (O : OBdd
         intro j hj1 hj2
         have := (hhp _).1 _ hl
         rw [hj2] at this
-        have that := (invh.2 _ (.inr j) this).1 _ hj1 rfl
+        have that := (invh.2 _ (.node j) this).1 _ hj1 rfl
         simp only at that
         rw [that]
         exact aux_lt2_low O_root_def U_root_def
